J_{r_1} 	&= k(X)(X_{c_6} X_{c_21}  - K_{r_1}X_{c_5} )\\
J_{r_2} 	&= k(X)(X_{c_5}  - K_{r_2}X_{c_7} )\\
J_{r_3} 	&= k(X)(X_{c_7}  - K_{r_3}X_{c_8} )\\
J_{r_4} 	&= k(X)(X_{c_3} X_{c_8}  - K_{r_4}X_{c_1} X_{c_9} )\\
J_{r_5} 	&= k(X)(X_{c_9}  - K_{r_5}X_{c_10} X_{c_11} )\\
J_{r_6} 	&= k(X)(X_{c_11}  - K_{r_6}X_{c_10} )\\
J_{r_7} 	&= k(X)(X_{c_6} X_{c_11} X_{c_20}  - K_{r_7}X_{c_2} X_{c_12} )\\
J_{r_8} 	&= k(X)(X_{c_1} X_{c_12}  - K_{r_8}X_{c_3} X_{c_13} )\\
J_{r_9} 	&= k(X)(X_{c_13}  - K_{r_9}X_{c_14} )\\
J_{r_10} 	&= k(X)(X_{c_14}  - K_{r_10}X_{c_18} )\\
J_{r_11} 	&= k(X)(X_{c_1} X_{c_18}  - K_{r_11}X_{c_3} X_{c_19} )\\
J_{r_12} 	&= k(X)(X_{c_2} X_{c_19}  - K_{r_12}X_{c_15} X_{c_20} )\\
J_{r_13} 	&= k(X)(X_{c_3} X_{c_16}  - K_{r_13}X_{c_1} X_{c_4} )\\
J_{r_14} 	&= k(X)(X_{c_3} X_{c_17}  - K_{r_14}X_{c_1}^{2} )\\
J_{r_15} 	&= k(X)(X_{c_3}  - K_{r_15}X_{c_1} X_{c_6} )\\
J_{r_16} 	&= k(X)(X_{c_15}  - K_{r_16}X_{c_22} )\\
